\documentclass[a4paper]{article}
\usepackage[utf8]{inputenc}
\usepackage{amsmath}
\usepackage{amsfonts}
\usepackage{amssymb}
\setlength{\parindent}{0in}
\usepackage{fancyhdr}

\begin{document}

\pagestyle{fancy}
\rhead{David Nápravník - přezdívka ":)"}

\section{du}
\subsection{}
\subsubsection{$(a_n) = (1, -1, 2, -1, 3, -3, ...)$}
$
(a_n) = (1, 0, 2, 0, 3, 0 ...) - (0, 1, 0, 2, 0, 3) + (0, 0, 0, 1, 0, 0 ...)\\
f(x) = 	\frac{1-x}{(1-x^2)^2} + x^3	
$

\subsubsection{$(b_n) = (1, -3, 5, -7, 9, -11, ...)$}
prohodíme $-x$ za $x$, přičteme $(1, 1, 1, ...)$ a vydělíme 2
\\ \\
$
\sum_{n \geq 0}(2n + 1)x^n = 
\frac{1-x}{(1+x)^2}
$


\subsubsection{$(c_n) = (1, 4, 9, 16, 25, 36, ...)$}
$
\sum_{n \geq 0} n^2 x^n =
\frac{2}{(1-x)^3} - \frac{3}{(1-x)^2} + \frac{1}{1-x} = 
\frac{x(x+1)}{(1-x)^3}
$

\subsection{}
\subsubsection{$[x^5] : (2x - 1)^-2$}
$
\frac{1}{(1-2x)^2}=
\sum_{n=0}^\infty x^n 2^n (1+n)
\\ \\
\left[ x^5 \right] : 192
$

\subsubsection{$[x^5] : (1 + x)^{-1/3}$}
$
\sum_{n=0}^\infty \binom{-\frac{1}{3}}{n} x^n
\\ \\
\left[ x^5 \right] : -\frac{91}{729}
$


\subsection{}
\subsubsection{$a_0 = 0, a_1 = 1, a_n = a_{n-1} + a_{n-2} + 2$}
$
a_0 \rightarrow (0, 1, f_1 + f_2 + 2, ...)\\
=(0, 1, 0, 0 ...) = x \\
+(0, f_0, f_1, f_2, ...) = x f(x)\\
+(0, 0, f_0, f_1, ...) = x^2 f(x)\\ 
+(0, 0, 2,2, ...) = \frac{2x^2}{1-x}
\\ \\
f(x)= x+xf(x)+x^2f(x)+\frac{2x^2}{1-x} \\
1=\frac{x}{f(x)}+x+x^2+\frac{\frac{2x^2}{1-x}}{f(x)} \\
f(x) = \frac{x+\frac{2x^2}{1-x}}{1-x-x^2} \\
\rightarrow x\neq\frac{-1-\sqrt{5}}{2}, x\neq\frac{\sqrt{5}-1}{2}, x\neq1\\
\\
a_n = \left(-2+\frac{2^{-n}\left((1-\sqrt{5})^n(-2+\sqrt{5})+(1+\sqrt{5})^n(2+\sqrt{5})\right)}{\sqrt{5}}\right)
$

\subsubsection{$b_0 = 2, b_1 = 3, b_n = 3b_{n-2} - 2b_{n-1}$}
$
a_0 \rightarrow (2, 3, 3f_0 - 2f_1)\\
= (2, 3, 0, 0) = 2 + 3x\\
+ (0, 0, 3f_0, 3f_1) = 3x^2f(x)\\
+ (0, 0, -2f_1, -2f_2) = -2xf(x) + 4x\\
\\
f(x) = 2 + 3x + 3x^2f(x)  - 2f(x) + 4x\\
f(x)-3x^2f(x)+2xf(x) = 2 + 7x \\
1-3x^2+2x = \frac{2 + 7x}{f(x)}\\
f(x) = \frac{2 + 7x}{1-3x^2+2x }\\
\rightarrow x\neq-\frac{1}{3}, x\neq1 \\
\\
a_n = \frac{9-(-3)^n}{4}
$


\end{document}